\section{Appendix}

%% \subsection{Justifications}
%% \begin{align}
%%   \label{justification:lhospital}
%%   \lim_{x \to 0} x\log{x} & = \lim_{x \to 0} {\log{x} \over {1 \over x}} \\
%%                           & = \lim_{x \to 0} {{1 \over x} \over {-1 \over x^2}}\\
%%                           & = \lim_{x \to 0} {-x^2 \over x} \\
%%                           & = \lim_{x \to 0} -x \\
%%                           & = 0
%% \end{align}

\subsection{Optimization Dynamics}
\label{sec:proof-for-jsd-thing}
\begin{small}
  \begin{align}
    & \mathbb{E}\left[\log{{\ptx \over \pgx + \ptx}}\right] + \mathbb{E}\left[\log{\pgx\over\pgx + \ptx}\right] + \log4 - \log4 \\
    & = \sum_{x}\ptx\log{\ptx \over \pgx + \ptx} + \sum_{x}\pgx\log{\pgx \over \pgx + \ptx} + \log4 - \log4 \\
    & = \sum_{x}\ptx\log{\ptx \over \pgx + \ptx} + \sum_{x}\pgx\log{\pgx \over \pgx + \ptx} + \log2 + \log2 - \log4 \\
    & = \sum_{x}\ptx\log{\ptx \over \pgx + \ptx} + \sum_{x}\pgx\log{\pgx
      \over \pgx + \ptx} \\
    & \quad + \sum_{x}\ptx\log2 + \sum_{x}\pgx\log2 - \log4 \\
    & = \sum_{x}\ptx\log{2\ptx \over \pgx + \ptx} + \sum_{x}\pgx\log{2\pgx \over \pgx + \ptx} - \log4 \\
    & = \sum_{x}\ptx\log{\ptx \over {\pgx + \ptx \over 2}} + \sum_{x}\pgx\log{\pgx \over {\pgx + \ptx \over 2}} - \log4 \\
    & = \KL{\ptx}{\pgx + \ptx \over 2} + \KL{\pgx}{\pgx+\ptx \over 2} - \log4 \\
    & = 2 \cdot \JSD{\pgx}{\ptx} - \log4
  \end{align}
\end{small}

%% \subsection{Minimax and Maximin}
%% \subsubsection{Minimax of $\VD$}
%% \begin{align}
%%   \overline{\VD} & = \min_{\mathbf{\phi}}\max_{\mathbf{\theta}}
%%                    V_{\D}(\theta, \phi) \\
%%                  & = \min_{\mathbf{\phi}}\max_{\mathbf{\theta}} \left (
%%                    \mathbb{E}\left[\log{\D(x)}\right] +
%%                    \mathbb{E}\left[\log(1 -
%%                    \D(\G(\mathbf{z})))\right] \right) \\
%%                  & = \min_{\mathbf{\phi}}\left(\max_{\mathbf{\theta}} \left (
%%                    \mathbb{E}\left[\log{\D(x)}\right] +
%%                    \mathbb{E}\left[\log(1 -
%%                    \D(\G(\mathbf{z})))\right] \right)
%%                    \right) \\
%%                  & = \min_{\phi}\left(\mathbb{E}\left[\log{\pt \over
%%                    \pg + \pt}\right] + \mathbb{E}\left[\log\left(1 - {\pt \over
%%                    \pg + \pt}\right)\right] \right) \\
%%                  & = \mathbb{E}\left[\log{\pt \over \pt + \pt}\right] +
%%                    \mathbb{E}\left[\log\left(1 - {\pt \over
%%                    \pt + \pt}\right)\right] \\
%%                  & = \mathbb{E}\left[\log{1 \over 2}\right] +
%%                    \mathbb{E}\left[\log{\left(1 - {1 \over 2}\right)}\right] \\
%%                  & = \log{1 \over 2} + \log{1 \over 2} \\
%%                  & = \log{1 \over 4}.
%% \end{align}
%%
%% \subsubsection{Maximin of $\VD$}
%%
%% \begin{align}
%%   \underline{\VD} & =
%%                     \max_{\mathbf{\theta}}\min_{\mathbf{\phi}}V_{\D}(\theta,
%%                     \phi) \\
%%                   & =
%%                     \max_{\mathbf{\theta}}\min_{\mathbf{\phi}} \left(
%%                     \mathbb{E}\left[\log{\D(x)}\right] +
%%                     \mathbb{E}\left[\log(1 - \D(\G(\mathbf{z})))\right]\right) \\
%%                   & = \max_{\mathbf{\theta}}\left(\min_{\mathbf{\phi}} \left(
%%                     \mathbb{E}\left[\log{\D(x)}\right] +
%%                     \mathbb{E}\left[\log(1 -
%%                     \D(\G(\mathbf{z})))\right]\right)\right) \\
%%                   & = \max_{\mathbf{\theta}}\left(\left(
%%                     \mathbb{E}\left[\log{\D(x)}\right] +
%%                     \mathbb{E}\left[\log(1 -
%%                     \D(x))\right]\right)\right) \\
%%                   & = \max_{\mathbf{\theta}}\left(\left(
%%                     \mathbb{E}\left[\log{\D(x)} +
%%                     \log(1 - \D(x))\right]\right)\right) \\
%%                   & = \mathbb{E}\left[\log{\pt \over \pt + \pt}\right]
%%                     + \mathbb{E}\left[\log\left(1 - {\pt \over \pt + \pt}\right)\right] \\
%%                   & = \mathbb{E}\left[\log{1 \over 2}\right] + \mathbb{E}\left[\log{\left(1 - {1 \over 2}\right)}\right] \\
%%                   & = \log{1 \over 2} + \log{1 \over 2} \\
%%                   & = \log{1 \over 4}.
%% \end{align}
%%
%% \subsubsection{Minimax of $\VG$}
%%
%% \begin{align}
%%   \overline{\VG} & = \min_{\theta}\max_{\phi} \VG \\
%%                  & = \min_{\theta}\max_{\mathbf{\phi}}
%%                    \left (-\mathbb{E}\left[\log{\D(x)}\right] -
%%                    \mathbb{E}\left[\log(1 -
%%                    \D(\G(\mathbf{z})))\right] \right) \\
%%                  & = \min_{\theta}\left(\max_{\mathbf{\phi}}
%%                    \left (-\mathbb{E}\left[\log{\D(x)}\right] -
%%                    \mathbb{E}\left[\log(1 -
%%                    \D(\G(\mathbf{z})))\right] \right)
%%                    \right) \\
%%                  & = \min_{\theta}\left(
%%                    -\mathbb{E}\left[\log{\D(x)}\right] -
%%                    \mathbb{E}\left[\log(1 -
%%                    \D(x))\right] \right) \\
%%                  & = \min_{\theta}\left(
%%                    -\mathbb{E}\left[\log{\D(x)} +
%%                    \log(1 - \D(x))\right] \right) \\
%%                  & = -\mathbb{E}\left[\log{\pt \over \pt + \pt} +
%%                    \log\left(1 - {\pt \over \pt + \pt}\right)\right] \\
%%                  & = - \mathbb{E}\left[\log{1 \over 2} +
%%                    \log{\left(1 - {1 \over 2}\right)}\right] \\
%%                  & = - \log{1 \over 2} - \log{1 \over 2} \\
%%                  & = - \log{1 \over 4}.
%% \end{align}
%%
%% \subsubsection{Maximin of $\VG$}
%%
%% \begin{align}
%%   \underline{\VG} & = \max_{\mathbf{\phi}} \min_{\mathbf{\theta}}\VG \\
%%                   & = \max_{\mathbf{\phi}}\min_{\mathbf{\theta}}\VG \\
%%                   & = \max_{\phi}\min_{\theta} \left(
%%                     -\mathbb{E}\left[\log{\D(x)}\right] -
%%                     \mathbb{E}\left[\log(1 -
%%                     \D(\G(\mathbf{z})))\right] \right) \\
%%                   & = \max_{\phi}\left(\min_{\theta} \left(
%%                     -\mathbb{E}\left[\log{\D(x)}\right] -
%%                     \mathbb{E}\left[\log(1 -
%%                     \D(\G(\mathbf{z})))\right] \right)
%%                     \right) \\
%%                   & = \max_{\phi}\left(
%%                     -\mathbb{E}\left[\log{\pt \over \pt + \pg} +
%%                     \log(1 -
%%                     {\pt \over \pt + \pg}\right] \right) \\
%%                   & =
%%                     -\mathbb{E}\left[\log{\pt \over \pt + \pt} +
%%                     \log(1 -
%%                     {\pt \over \pt + \pt})\right] \\
%%                  & = - \mathbb{E}\left[\log{1 \over 2} +
%%                    \log{\left(1 - {1 \over 2}\right)}\right] \\
%%                  & = - \log{1 \over 2} - \log{1 \over 2} \\
%%                  & = - \log{1 \over 4}.
%% \end{align}





%%% Local Variables:
%%% mode: latex
%%% TeX-master: "../thesis"
%%% End:
